Progress on LRU cache

Test/tutorial/LRU_cache/two.dfy
@@ -3,33 +3,29 @@ datatype Outcome<T> =
 	| Failure
 
 datatype entry<T> = Entry(key: nat,value: T)
-
-// There are different approaches to the formalization
-
-// One possibility is to define the log so that it contains the trace of all operations
-// Then the properties are "intemporal": you can say, at any index, if the entry is a get
-// then ...
-
 	
 trait Storage<T(!new)> {
 
 	ghost var log: seq<entry<T>>
-	
-	// function method get(key: nat): Outcome<T>
-	// 	reads this
+
+	predicate Invariant()
+		reads this
+
+	method get(key: nat) returns (result: Outcome<T>)
+		requires Invariant()
+		ensures Invariant()
+		ensures result.Success? <==> exists index: nat :: index < |log| && log[index].key == key
+		ensures result.Failure? <==> !exists index: nat :: index < |log| && log[index].key == key
 		
-	// method put(key: nat, value: T)
-	// 	modifies this
-	// 	ensures log == old(log) + [Entry(key,value)]
-
-	// lemma prop1(key: nat, result: Outcome<T>)
-	// 	requires get(key) == result
-	// 	requires result.Success?
-	// 	ensures exists index: nat :: index < |log| && log[index] == Entry(key,result.value) && (forall index': nat :: index' > index && index' < |log| ==> log[index'].key != key)
-
-	// lemma prop2(key: nat)
-	// 	requires get(key).Failure?
-	// 	ensures forall index: nat :: index < |log| ==> log[index].key != key
+	function method fget(key: nat): Outcome<T>
+ 		reads this
+		requires Invariant()
+		
+	method put(key: nat, value: T)
+	 	modifies this
+		requires Invariant()
+		ensures log == old(log) + [Entry(key,value)]
+		ensures Invariant()
 		
 }
 
@@ -37,54 +33,48 @@ class MapStorage<T(!new)> extends Storage<T> {
 
 	var storage: map<nat,T>
 
-	predicate InSync()
+	predicate Invariant()
 		reads this
 	{
-		forall key: nat :: key in storage ==> exists index: nat :: index < |log| && log[index].key == key
+		&& forall key: nat :: key in storage <==> exists index: nat :: index < |log| && log[index].key == key
 	}
 	
 	constructor()
-		ensures InSync()
+		ensures Invariant()
 	{
 		storage := map[];
 		log := [];
 	}
 
-	method get1(key: nat) returns (result: Outcome<T>)
-		requires InSync()
-		ensures InSync()
-		ensures result.Success? ==> exists index: nat :: index < |log| && log[index].key == key
+	method get(key: nat) returns (result: Outcome<T>)
+		requires Invariant()
+		ensures Invariant()
+		ensures result.Success? <==> exists index: nat :: index < |log| && log[index].key == key
+		ensures result.Failure? <==> !exists index: nat :: index < |log| && log[index].key == key
 	{
 		if key in storage {
 			result := Success(storage[key]);
-			//ghost var index: nat :| index < |log| && log[index].key == key;
 		} else {
 			result := Failure;
 		}
 	}
-	
-	function method get2(key: nat): Outcome<T>
-		reads this
-	{
-		if key in storage then Success(storage[key]) else Failure
-	}
 
 	method put(key: nat, value: T)
 		modifies this
-		requires InSync()
+		requires Invariant()
 		ensures log == old(log) + [Entry(key,value)]
-		ensures InSync()
+		ensures Invariant()
 	{
 
-		assert forall key: nat :: key in storage ==> exists index: nat :: index < |log| && log[index].key == key;
+		assert forall key: nat :: key in storage <==> exists index: nat :: index < |log| && log[index].key == key;
 
 		storage := storage[key := value];
 
-		assert forall key: nat :: key in old(storage) ==> exists index: nat :: index < |log| && log[index].key == key;
+		assert forall key: nat :: key in old(storage) <==> exists index: nat :: index < |log| && log[index].key == key;
 
 		log := log + [Entry(key,value)];
 
-		assert forall key: nat :: key in old(storage) ==> exists index: nat :: index < |old(log)| && old(log)[index].key == key;
+		assert forall key: nat :: key in old(storage) <==> exists index: nat :: index < |old(log)| && old(log)[index].key == key;
 
 		forall key': nat ensures key' in storage ==> exists index: nat :: index < |log| && log[index].key == key' {
 			if key' in storage {
@@ -100,21 +90,18 @@ class MapStorage<T(!new)> extends Storage<T> {
 		}
 	}
 
-	// lemma test(key: nat, result: Outcome<T>)
-	// 	requires get2(key) == result
-	// 	requires result.Success?
-	// 	ensures exists index: nat :: index < |log| && log[index].key == key
-	// {
-		
-	// }
+	function method fget(key: nat): Outcome<T>
+		reads this
+		requires Invariant()
+	{
+		if key in storage then Success(storage[key]) else Failure
+	}
 	
-	// lemma prop1(key: nat, result: Outcome<T>)
-	// 	requires get(key) == result
-	// 	requires result.Success?
-	// 	ensures exists index: nat :: index < |log| && log[index] == Entry(key,result.value) && (forall index': nat :: index' > index && index' < |log| ==> log[index'].key != key)
-		
-	// lemma prop2(key: nat)
-	// 	requires get(key).Failure?
-	// 	ensures forall index: nat :: index < |log| ==> log[index].key != key
+	lemma prop_test_1(key: nat)
+		requires Invariant()
+		requires fget(key).Success?
+		ensures exists index: nat :: index < |log| && log[index].key == key
+	{
+	}
 
 }
